Veritas.SeqMachine.fst
@@ -1,0 +1,129 @@
+module Veritas.SeqMachine
+
+open FStar.Seq
+open Veritas.SeqAux
+
+let lemma_empty_seq_valid (sm: seq_machine):
+  Lemma (valid sm (empty #(elem_type sm))) =
+  lemma_reduce_empty (init_state sm) (trans_fn sm)
+
+let lemma_valid_prefix (sm: seq_machine) (s: (seq (elem_type sm)){valid sm s}) (i:nat{i <= length s}):
+  Lemma (valid sm (prefix s i)) =
+  let si = prefix s i in
+  if valid sm si then ()
+  else (
+    lemma_reduce_prefix (init_state sm) (trans_fn sm) s i;
+    lemma_reduce_identity (fail_state sm) (trans_fn sm) (suffix s (length s - i))
+  )
+
+let rec max_valid_prefix_aux (sm: seq_machine) (s: seq (elem_type sm))
+  : Tot (i:nat{i <= length s /\
+              valid sm (prefix s i) /\
+              (i < length s ==> not (valid sm (prefix s (i + 1))))
+              })
+    (decreases (length s)) =
+  lemma_empty_seq_valid sm;
+  lemma_prefix0_empty s;
+  let n = length s in
+  if valid sm s then n
+  else max_valid_prefix_aux sm (prefix s (n - 1))
+
+let max_valid_prefix = max_valid_prefix_aux
+
+let lemma_empty_seq_valid_all (psm: pseq_machine):
+  Lemma (valid_all psm (empty #(elem_type_p psm))) =
+  let s = empty #(elem_type_p psm) in
+  let key = key_type psm in
+  let sm = seq_machine_of psm in
+  let pf = partn_fn psm in
+  let iskey (k: key) = fun e -> pf e = k in
+  let aux(k: key):
+    Lemma (requires True)
+          (ensures (valid sm (filter (fun e -> pf e = k) s)))
+          [SMTPat (valid sm (filter (iskey k) s))]
+          =
+    lemma_filter_empty (iskey k);
+    lemma_empty_seq_valid sm
+  in
+  ()
+
+let lemma_valid_all_prefix (psm: pseq_machine)
+                           (s: (seq (elem_type_p psm)){valid_all psm s}) (i:nat{i <= length s}):
+  Lemma (requires True)
+        (ensures (valid_all psm (prefix s i)))
+        (decreases (length s)) =
+  let si = prefix s i in
+  let key = key_type psm in
+  let sm = seq_machine_of psm in
+  let pf = partn_fn psm in
+  let iskey (k: key) = fun e -> pf e = k in
+  let aux(k: key):
+    Lemma (requires True)
+          (ensures (valid sm (filter (iskey k) si)))
+          [SMTPat (valid sm (filter (iskey k) si))]
+    =
+    lemma_filter_prefix (iskey k) s si;
+    lemma_valid_prefix sm (filter (iskey k) s) (length (filter (iskey k) si))
+  in
+  ()
+
+(* for some reason fstar requires this trivial lemma in the proof below *)
+let lemma_not_valid_k (psm: pseq_machine) (k: (key_type psm)) (s: seq (elem_type_p psm)):
+  Lemma (requires (~ (valid (seq_machine_of psm) (filter (fun e -> (partn_fn psm e) = k) s))))
+        (ensures (~ (valid_all psm s))) = ()
+
+let lemma_valid_all_extend (psm: pseq_machine) (s: seq (elem_type_p psm)):
+  Lemma (requires (length s > 0 /\
+                   valid_all psm (prefix s (length s - 1)) /\
+                   valid (seq_machine_of psm)
+                         (filter (fun e -> (partn_fn psm e) = (partn_fn psm (index s (length s - 1)))) s)))
+        (ensures (valid_all psm s)) =
+  let n = length s in
+  let sm = seq_machine_of psm in
+  let pf = partn_fn psm in
+  let key = key_type psm in
+  let iskey (k: key) = fun e -> pf e = k in
+  let k' = pf (index s (n - 1)) in
+  let aux(k: key):
+    Lemma (requires True)
+          (ensures (valid sm (filter (iskey k) s)))
+          [SMTPat (valid sm (filter (iskey k) s))] =
+    if k' = k then lemma_filter_extensionality (iskey k') (iskey k) s
+    else lemma_filter_extend1 (iskey k) s
+  in
+  ()
+
+let rec max_valid_all_prefix_aux (psm: pseq_machine) (s: seq (elem_type_p psm))
+  : Tot (i: nat{i <= length s /\
+               valid_all psm (prefix s i) /\
+               (i < length s ==>
+                ~ (valid_all psm (prefix s (i + 1))))})
+    (decreases (length s)) =
+  let n = length s in
+  let sm = seq_machine_of psm in
+  let pf = partn_fn psm in
+  let key = key_type psm in
+  let iskey (k: key) = fun e -> pf e = k in
+  if n = 0 then (
+    lemma_prefix0_empty s;
+    lemma_empty_seq_valid_all psm;
+    0
+  )
+  else 
+    let s' = prefix s (n - 1) in
+    let i = max_valid_all_prefix_aux psm s' in
+    if i = n - 1 then
+      let e = index s (n - 1) in
+      let k = pf e in
+      let sk = filter (iskey k) s in
+      if valid sm sk then (
+        lemma_valid_all_extend psm s;
+        n
+      )
+      else (
+        lemma_not_valid_k psm k s;
+        i
+      )    
+    else i
+  
+let max_valid_all_prefix = max_valid_all_prefix_aux
