Veritas.SeqMachine.fsti
@@ -1,0 +1,96 @@
+module Veritas.SeqMachine
+
+open FStar.Seq
+open Veritas.SeqAux
+
+(* a transition function tr is failure propagating
+ * if it remains in failure state once entered
+ *)
+let failure_prop_fn (#a:eqtype) (#st:eqtype) (sf:st) (tr:a -> st -> st) 
+  = forall (a1:a). tr a1 sf = sf
+
+noeq type seq_machine = 
+  | SeqMachine: #a:eqtype ->                                  // elements of sequence
+                #st:eqtype ->                               // state type
+                s0:st ->                                    // initial state
+                sf:st{sf <> s0} ->                           // final state
+                tr: (a -> st -> st){failure_prop_fn sf tr}  // transition function
+                -> seq_machine
+
+let elem_type (sm: seq_machine) = 
+  match sm with
+  | SeqMachine #a #_ _ _ _ -> a
+
+let state_type (sm: seq_machine) = 
+  match sm with 
+  | SeqMachine #_ #s _ _ _ -> s
+
+let init_state (sm: seq_machine): Tot (state_type sm) = 
+  match sm with 
+  | SeqMachine s0 _ _ -> s0
+
+let fail_state (sm: seq_machine): Tot (state_type sm) = 
+  match sm with
+  | SeqMachine _ sf _ -> sf
+
+let trans_fn (sm: seq_machine): 
+  Tot (tr: ((elem_type sm) -> (state_type sm) -> (state_type sm))
+           {failure_prop_fn (fail_state sm) tr}) = 
+  match sm with
+  | SeqMachine _ _ tr -> tr
+
+(* run the seq machine on a sequence *)
+let seq_machine_run (sm: seq_machine) (s: seq (elem_type sm)): Tot (state_type sm) = 
+  reduce (init_state sm) (trans_fn sm) s
+
+(* validity: we donot end up with the failure state *)
+let valid (sm: seq_machine) (s: seq (elem_type sm)) = 
+  (fail_state sm) <> (seq_machine_run sm s)
+
+(* empty sequence is valid *)
+val lemma_empty_seq_valid (sm: seq_machine):
+  Lemma (valid sm (empty #(elem_type sm)))
+
+val lemma_valid_prefix (sm: seq_machine) (s: (seq (elem_type sm)){valid sm s}) (i:nat{i <= length s}):
+  Lemma (valid sm (prefix s i))
+
+(* the maximum valid prefix of a sequence is computable *)
+val max_valid_prefix (sm: seq_machine) (s: seq (elem_type sm))
+  : Tot (i:nat{i <= length s /\ 
+              valid sm (prefix s i) /\
+              (i < length s ==> not (valid sm (prefix s (i + 1))))
+              })
+
+(* partitioned seq_machine *)
+noeq type pseq_machine =
+  | PSM: #key:eqtype -> sm: seq_machine -> pf: ((elem_type sm) -> key) -> pseq_machine
+
+let seq_machine_of (psm: pseq_machine) = 
+  match psm with
+  | PSM sm _ -> sm
+
+let key_type (psm: pseq_machine): eqtype = 
+  match psm with
+  | PSM #k _ _ -> k
+
+let elem_type_p (psm: pseq_machine) = elem_type (seq_machine_of psm)
+
+let partn_fn (psm: pseq_machine): (elem_type_p psm -> key_type psm)  = 
+  match psm with
+  | PSM _ pf -> pf
+
+let valid_all (psm: pseq_machine) (s: seq (elem_type_p psm)) = 
+  forall (k:(key_type psm)). valid (seq_machine_of psm) (filter (fun e -> (partn_fn psm e) = k) s)
+
+val lemma_empty_seq_valid_all (psm: pseq_machine):
+  Lemma (valid_all psm (empty #(elem_type_p psm)))
+
+val lemma_valid_all_prefix (psm: pseq_machine) 
+                           (s: (seq (elem_type_p psm)){valid_all psm s}) (i:nat{i <= length s}):
+  Lemma (valid_all psm (prefix s i))
+
+val max_valid_all_prefix (psm: pseq_machine) (s: seq (elem_type_p psm))
+  : Tot (i: nat{i <= length s /\
+               valid_all psm (prefix s i) /\
+               (i < length s ==> ~ (valid_all psm (prefix s (i + 1))))})
+
